ram-linear-time/proofs/Lax11Proofs.lean
@@ -4,3 +4,4 @@ import Lax11Proofs.Labels
 import Lax11Proofs.Imp
 import Lax11Proofs.Machine
 import Lax11Proofs.Compile
+import Lax11Proofs.Simulation
